src/Renaming2.v
@@ -1,11 +1,12 @@
-Require Import Setoid Morphisms Morph Var2.
+Require Import Setoid Morphisms StrictProp
+        Morph Index Name Level Var2.
 
 (* Algebra of operations on [var 0] *)
-Inductive renaming (trm : Set) :=
+Inductive renaming (trm : nset) :=
 | r_id
 | r_shift (b : name) (r : renaming trm)
 | r_rename (b : name) (r : renaming trm) (a : name)
-| r_subst (t : trm) (r : renaming trm) (a : name).
+| r_subst (t : trm 0) (r : renaming trm) (a : name).
 
 Arguments r_id {trm}.
 Arguments r_shift {trm} b r.
@@ -32,50 +33,122 @@ Notation "r , a" := (r_rename a r a)
 Delimit Scope ren_scope with ren.
 *)
 
-Fixpoint static {trm : Set} (r : renaming trm) : Prop :=
+Section Apply.
+
+  Context {trm : nset}.
+
+  Variable unit : forall {N}, ivar N (@trm) N.
+
+  Variable kleisli :
+    forall {N M},
+      ivar N (@trm) M ->
+      morph (@trm) N (@trm) M.
+
+  Fixpoint apply_renaming (r : renaming trm) {N M}
+  : static r -> ivar N T M -> ivar N T M :=
+  match r return static r -> ivar N T M -> ivar N T M with
+  | r_id => fun _ f => f
+  | r_shift b r =>
+      fun s f =>
+        weak_ivar (apply_static_ivar r s (open_ivar b f))
+  | r_rename b r a =>
+      fun s f =>
+        close_ivar a (apply_static_ivar r s (open_ivar b f))
+  | r_subst _ r _ => sEmpty_rect _
+  end.
+  Arguments apply_static_ivar {T} r {N M} s f.
+
+End Apply.
+
+Section RenamingRelativeMonad.
+
+  Parameter term : forall {V : nat}, Set.
+
+  Parameter unit : forall {N}, morph (@var) N (@term) N.
+
+  Parameter kleisli :
+    forall {N M},
+      morph (@var) N (@term) M ->
+      morph (@term) N (@term) M.
+
+  Axiom left_identity :
+    forall N M (f : morph (@var) N (@term) M) V t,
+      kleisli f V (unit V t) = f V t.
+
+  Axiom right_identity :
+    forall N V (t : @term (N + V)),
+      kleisli unit V t = t.
+
+  Axiom associativity :
+    forall N M L
+      (f : morph (@var) N (@term) M)
+      (g : morph (@var) M (@term) L) V t,
+      kleisli (fun V' t' => kleisli g V' (f V' t')) V t
+      = kleisli g V (kleisli f V t).
+
+  Axiom unit_extend :
+    forall N V v,
+      morph_extend (@unit N) V v = unit V v.
+
+  Axiom kleisli_extend :
+    forall N M (f : morph (@var) N (@term) M) V t,
+      morph_extend (kleisli f) V t
+      = kleisli (morph_extend f) V t.
+
+  Axiom extensional :
+    forall N M (f g : morph (@var) N (@term) M) V t,
+      (forall V t, f V t = g V t) ->
+      kleisli f V t = kleisli g V t.
+
+
+
+
+Fixpoint static {T : nset} (r : renaming T) : SProp :=
   match r with
-  | r_id => True
+  | r_id => sUnit
   | r_shift b r => static r
   | r_rename b r a => static r
-  | r_subst u r a => False
+  | r_subst u r a => sEmpty
   end.
 
-Fixpoint apply_static_ivar {trm} (r : renaming trm)
-         {N T M} (f : ivar N T M) : ivar N T M :=
-  match r with
-  | r_id => f
+Fixpoint apply_static_ivar {T} (r : renaming T) {N M}
+  : static r -> ivar N T M -> ivar N T M :=
+  match r return static r -> ivar N T M -> ivar N T M with
+  | r_id => fun _ f => f
   | r_shift b r =>
-      weak_ivar (apply_static_ivar r (open_ivar b f))
+      fun s f =>
+        weak_ivar (apply_static_ivar r s (open_ivar b f))
   | r_rename b r a =>
-      close_ivar a (apply_static_ivar r (open_ivar b f))
-  | r_subst _ r _ => apply_static_ivar r f
+      fun s f =>
+        close_ivar a (apply_static_ivar r s (open_ivar b f))
+  | r_subst _ r _ => sEmpty_rect _
   end.
+Arguments apply_static_ivar {T} r {N M} s f.
 
-Add Parametric Morphism {trm r N} {T : nset} {M}
-  : (@apply_static_ivar trm r N T M)
+Add Parametric Morphism {T r N M s}
+  : (@apply_static_ivar T r N M s)
     with signature eq_morph ==> eq_morph
     as sapply_ivar_mor.
   generalize dependent M.
-  generalize dependent T.
   generalize dependent N.
   induction r; intros * Heq; cbn.
   - easy.
-  - rewrite IHr with (y := open_ivar b y) by (rewrite Heq; easy).
+  - rewrite IHr with (y := open_ivar b y)
+      by (rewrite Heq; easy).
     easy.
-  - rewrite IHr with (y := open_ivar b y) by (rewrite Heq; easy).
+  - rewrite IHr with (y := open_ivar b y)
+      by (rewrite Heq; easy).
     easy.
-  - rewrite IHr with (y := y) by (rewrite Heq; easy).
-    easy.
+  - easy.
 Qed.
 
-Lemma snd_apply_static_ivar {trm N T M} (r : renaming trm)
+Lemma snd_apply_static_ivar {N T M} (r : renaming T)
       (f : ivar N T M) :
   snd_ivar (apply_static_ivar r f) = snd_ivar f.
 Proof.
   generalize dependent M.
-  generalize dependent T.
   generalize dependent N.
-  induction r; intros N T M f; cbn.
+  induction r; intros N M f; cbn.
   - easy.
   - simpl_ivars_pointwise.
     rewrite IHr; easy.
@@ -84,16 +157,15 @@ Proof.
   - easy.
 Qed.
 
-Lemma fst_apply_static_ivar {trm N T M} (r : renaming trm)
+Lemma fst_apply_static_ivar {N T M} (r : renaming T)
       (f : ivar N T M) (g : ivar N T M) :
   fst_ivar f =km= fst_ivar g ->
   fst_ivar (apply_static_ivar r f)
   =km= fst_ivar (apply_static_ivar r g).
 Proof.
   generalize dependent M.
-  generalize dependent T.
   generalize dependent N.
-  induction r; intros N T M f g Heq; cbn.
+  induction r; intros N M f g Heq; cbn.
   - easy.
   - simpl_ivars_pointwise.
     apply IHr.
@@ -109,34 +181,34 @@ Proof.
   - apply IHr; easy.
 Qed.
 
-Lemma swap_apply_static_ivar_transpose_ivar {trm N T M}
-      (r : renaming trm)
+Lemma transpose_swap_ivar_apply_static_ivar {N T M}
+      (r : renaming T)
       (f : ivar (S (S N)) T M) :
-  apply_static_ivar r (transpose_ivar f)
-  =m= transpose_ivar (apply_static_ivar r f).
+  swap_ivar (apply_static_ivar r f)
+  =m= apply_static_ivar r (swap_ivar f).
 Proof.
+  unfold swap_ivar; symmetry.
   rewrite <- ivar_eta_pointwise.
-  unfold transpose_ivar.
   rewrite snd_apply_static_ivar, snd_apply_static_ivar.
   rewrite fst_apply_static_ivar with (g := f) by easy.
   simpl_ivars_pointwise.
   easy.
 Qed.
 
-Fixpoint transfer_open_var {trm} (r : renaming trm) (a : name) :
-  name * renaming trm :=
+Fixpoint transfer_open_var {T} (r : renaming T) (a : name) :
+  name * renaming T :=
   match r with
   | r_id => pair a r_id
   | r_shift b r =>
       let ar' := transfer_open_var r a in
-      pair (shift_name b (fst ar'))
+      pair (shift_below_name b (fst ar'))
            (r_shift (unshift_name (fst ar') b) (snd ar'))
   | r_rename c r b =>
       match name_eqb a b with
       | true => pair c r
       | false =>
         let ar' := transfer_open_var r (unshift_name b a) in
-        pair (shift_name c (fst ar'))
+        pair (shift_below_name c (fst ar'))
              (r_rename (unshift_name (fst ar') c)
                        (snd ar')
                        (unshift_name a b))
@@ -146,20 +218,20 @@ Fixpoint transfer_open_var {trm} (r : renaming trm) (a : name) :
         pair (fst ar') (r_subst t (snd ar')  b)
   end.
 
-Lemma transfer_open_var_spec {trm} (r : renaming trm) a :
-  forall {N T M} (f : ivar N T M),
+Lemma transfer_open_var_spec {T} (r : renaming T) a :
+  forall {N M} (f : ivar N T M),
   open_ivar a (apply_static_ivar r f)
   =m= apply_static_ivar
         (snd (transfer_open_var r a))
         (open_ivar (fst (transfer_open_var r a)) f).
 Proof.
   generalize dependent a.
-  induction r; intros c N T M f; cbn in *.
+  induction r; intros c N M f; cbn in *.
   - easy.
-  - rewrite swap_open_ivar_weak_ivar_pointwise.
+  - rewrite transpose_open_ivar_weak_ivar_pointwise.
     rewrite IHr.
-    rewrite <- swap_apply_static_ivar_transpose_ivar.
-    rewrite swap_open_ivar_open_ivar_pointwise.
+    rewrite transpose_swap_ivar_apply_static_ivar.
+    rewrite transpose_open_ivar_open_ivar_pointwise.
     easy.
   - remember (name_eqb c a) as eq_ca eqn:Hca.
     symmetry in Hca.
@@ -168,17 +240,18 @@ Proof.
       simpl_ivars_pointwise.
       easy.
     + apply name_eqb_neq in Hca.
-      rewrite swap_open_ivar_close_ivar_pointwise by easy.
+      rewrite transpose_open_ivar_close_ivar_pointwise
+        by easy.
       rewrite IHr.
-      rewrite <- swap_apply_static_ivar_transpose_ivar.
-      rewrite swap_open_ivar_open_ivar_pointwise.
+      rewrite transpose_swap_ivar_apply_static_ivar.
+      rewrite transpose_open_ivar_open_ivar_pointwise.
       easy.
   - rewrite IHr.
     easy.
 Qed.
 
-Fixpoint compose_static {trm}
-         (r : renaming trm) (s : renaming trm) :=
+Fixpoint compose_static {T}
+         (r : renaming T) (s : renaming T) :=
   match r with
   | r_id => s
   | r_shift a r =>
@@ -194,21 +267,18 @@ Fixpoint compose_static {trm}
     r_subst t r' a
   end.
 
-Lemma compose_static_left_identity {trm} (r : renaming trm) :
+Lemma compose_static_left_identity {T} (r : renaming T) :
   compose_static r_id r = r.
 Proof. easy. Qed.
 
-Lemma compose_static_right_identity {trm} (r : renaming trm) :
+Lemma compose_static_right_identity {T} (r : renaming T) :
   compose_static r r_id = r.
 Proof.
-  induction r; cbn.
-  - easy.
-  - rewrite IHr; easy.
-  - rewrite IHr; easy.
-  - rewrite IHr; easy.
+  induction r; cbn; try rewrite IHr; easy.
 Qed.
 
-Lemma transfer_open_var_shift_name {trm} (r : renaming trm) a b :
+(*
+Lemma transfer_open_var_shift_name {T} (r : renaming T) a b :
   fst (transfer_open_var r (shift_name a b))
   = shift_name (fst (transfer_open_var r a))
       (fst (transfer_open_var (snd (transfer_open_var r a)) b)).
@@ -218,7 +288,7 @@ Proof.
   induction r; intros c d; cbn.
   - easy.
   - rewrite IHr.
-    rewrite swap_shift_name_shift_name.
+    rewrite transpose_shift_name_shift_name.
     easy.
   - remember (name_eqb c a) as eq_ca eqn:Hca.
     symmetry in Hca.
@@ -246,14 +316,14 @@ Proof.
         simpl_names; easy.
       * rewrite name_eqb_neq in Hdca.
         simpl_names; cbn.
-        rewrite <- swap_shift_name_shift_name.
+        rewrite <- transpose_shift_name_shift_name.
         rewrite <- IHr.
-        rewrite swap_unshift_name_shift_name by easy.
+        rewrite transpose_unshift_name_shift_name by easy.
         easy.
   - apply IHr.
 Qed.
 
-Lemma transfer_open_var_unshift_name {trm} (r : renaming trm) a b :
+Lemma transfer_open_var_unshift_name {T} (r : renaming T) a b :
   fst (transfer_open_var
          (snd (transfer_open_var r (shift_name a b)))
          (unshift_name b a))
@@ -271,7 +341,7 @@ Proof.
           (transfer_open_var
              (snd (transfer_open_var r c)) d)) as e.
     remember (fst (transfer_open_var r c)) as f.
-    rewrite swap_shift_name_unshift_name.
+    rewrite transpose_shift_name_unshift_name.
 
     
 
@@ -302,15 +372,15 @@ Proof.
         simpl_names; easy.
       * rewrite name_eqb_neq in Hdca.
         simpl_names; cbn.
-        rewrite <- swap_shift_name_shift_name.
+        rewrite <- transpose_shift_name_shift_name.
         rewrite <- IHr.
-        rewrite swap_unshift_name_shift_name by easy.
+        rewrite transpose_unshift_name_shift_name by easy.
         easy.
   - apply IHr.
 
-
-Lemma transfer_open_var_compose_static_fst {trm}
-      (r s : renaming trm) a :
+*)
+Lemma transfer_open_var_compose_static_fst {T}
+      (r s : renaming T) a :
    fst (transfer_open_var (compose_static r s) a)
    = fst (transfer_open_var s (fst (transfer_open_var r a))).
 Proof.
@@ -333,8 +403,8 @@ Proof.
   - apply IHr.
 Qed.
 
-Lemma transfer_open_var_compose_static_snd {trm}
-      (r s : renaming trm) a :
+Lemma transfer_open_var_compose_static_snd {T}
+      (r s : renaming T) a :
   snd (transfer_open_var (compose_static r s) a)
   = compose_static (snd (transfer_open_var r a))
       (snd (transfer_open_var s (fst (transfer_open_var r a)))).
@@ -360,7 +430,7 @@ Proof.
   - apply IHr.
 Qed.
 
-Lemma compose_static_associative {trm} (r s t : renaming trm) :
+Lemma compose_static_associative {T} (r s t : renaming T) :
   compose_static r (compose_static s t)
   = compose_static (compose_static r s) t.
 Proof.
@@ -375,7 +445,7 @@ Proof.
   - rewrite IHr; easy.
 Qed.
 
-Lemma apply_static_ivar_compose {trm N T M} (r : renaming trm) s
+Lemma apply_static_ivar_compose {T N T M} (r : renaming T) s
       (f : ivar N T M) :
   apply_static_ivar (compose_static r s) f
   =m= apply_static_ivar r (apply_static_ivar s f).
@@ -395,7 +465,7 @@ Proof.
   - easy.
 Qed.
 
-Fixpoint apply_static_var {trm} (r : renaming trm) : ivar 0 var 0 :=
+Fixpoint apply_static_var {T} (r : renaming T) : ivar 0 var 0 :=
   match r with
   | r_id => 1
   | r_shift b r =>
@@ -405,7 +475,7 @@ Fixpoint apply_static_var {trm} (r : renaming trm) : ivar 0 var 0 :=
   | r_subst _ r _ => apply_static_var r
   end.
 
-Lemma apply_static_ivar_as_composition {trm N T M} (r : renaming trm)
+Lemma apply_static_ivar_as_composition {T N T M} (r : renaming T)
       (f : ivar N T M) :
   apply_static_ivar r f =m=
   f @ (morph_extend_by N (apply_static_var r)).
@@ -427,7 +497,7 @@ Proof.
   - apply IHr.
 Qed.
 
-Lemma apply_static_var_spec {trm} (r : renaming trm) :
+Lemma apply_static_var_spec {T} (r : renaming T) :
   apply_static_var r =m= apply_static_ivar r 1.
 Proof.
   induction r; cbn.
@@ -441,8 +511,8 @@ Proof.
   - easy.
 Qed.
 
-Lemma apply_static_ivar_compose_distribute {trm N T M R L}
-      (r : renaming trm) (f : ivar N T M) (g : morph T M R L) :
+Lemma apply_static_ivar_compose_distribute {T N T M R L}
+      (r : renaming T) (f : ivar N T M) (g : morph T M R L) :
   g @ (apply_static_ivar r f)
   =m= apply_static_ivar r (g @ f).
 Proof.
@@ -453,7 +523,7 @@ Proof.
   easy.
 Qed.
 
-Lemma apply_static_var_compose {trm N T M} (r : renaming trm) s
+Lemma apply_static_var_compose {T N T M} (r : renaming T) s
       (f : ivar N T M) :
   apply_static_var (compose_static r s)
   =m= (apply_static_var s) @ (apply_static_var r).
